src/ReactorModel/Objects/Reactor/Core.lean
@@ -21,6 +21,9 @@ instance reactorType : ReactorType Reactor.Core where
   rcns  | mk _ _ _ r _ => r
   nest  | mk _ _ _ _ n => n
 
+instance : ReactorType.Extensional Reactor.Core where
+  ext_iff := by intro (mk ..) (mk ..); open ReactorType in simp [ports, state, rcns, acts, nest]
+
 instance : ReactorType.WellFounded Reactor.Core where
   wf := by
     constructor
